verify/boogie/auxiliary.bpl
@@ -42,9 +42,9 @@ type StateIndex = int;
 
 datatype Effect {
     // read(a,v,vis) == read at a the value v. vis means whether this read is visible to barriers
-    read(addr: int, read_value: int, read_visible: bool),
-    write(addr: int, write_value: int),
-    update(addr: int, read_value: int, read_visible: bool, write_value: int),
+    read(addr: bv64, read_value: bv64, read_visible: bool),
+    write(addr: bv64, write_value, write_mask: bv64),
+    update(addr: bv64, read_value: bv64, read_visible: bool, write_value, write_mask: bv64),
     no_effect()
 }
 
@@ -69,101 +69,73 @@ var ordering: [StateIndex] Ordering;
 
 
 
-// No implementation needed
-// Using explicit implementations makes it run very slow and it gives no extra information
-// The version without implementation creates a generic operation for each case
-// NOTE: There is an issue on the boogie repo with regards to this 
-function bit_and(x: int, y: int): int;
-function bit_or(x: int, y: int): int;
-function bit_xor(x: int, y: int): int;
 
-function bit_not(x: int): int;
+function {:bvbuiltin "bvshl"} shift_left(bv64,bv64) returns(bv64);
+function {:bvbuiltin "bvlshr"} shift_right(bv64,bv64) returns(bv64);
+function {:bvbuiltin "bvand"} bit_and(bv64,bv64) returns(bv64);
+function {:bvbuiltin "bvor"} bit_or(bv64,bv64) returns(bv64);
+function {:bvbuiltin "bvxor"} bit_xor(bv64,bv64) returns(bv64);
+function {:bvbuiltin "bvnot"} bit_inv(bv64) returns(bv64);
+function {:bvbuiltin "bvneg"} bin_neg(bv64) returns(bv64);
 
-axiom (forall x: int :: bit_not(bit_not(x)) == x); // double negation on bits
-axiom (forall x: int, y: int :: bit_and(x, y) == bit_and(y, x));
-axiom (forall x: int, y: int :: bit_or(x, y) == bit_or(y, x));
-axiom (forall x: int, y: int :: bit_xor(x, y) == bit_xor(y, x));
-axiom (forall x : int :: bit_and(0, x) == 0);
-axiom (forall x : int :: bit_or(x, 0) == x);
+function {:bvbuiltin "bvsub"} bin_sub(bv64,bv64) returns(bv64);
+function {:bvbuiltin "bvadd"} bin_add(bv64,bv64) returns(bv64);
 
-function shift_left(i : int, shift_amount : int) : int;
-function shift_right(i : int, shift_amount : int) : int;
-axiom (forall x : int :: shift_left(x, 0) == x);
-axiom (forall x : int :: shift_right(x, 0) == x);
-axiom (forall x : int :: shift_left(0, x) == 0);
-axiom (forall x : int :: shift_right(0, x) == 0);
+function {:bvbuiltin "bvule"} ule(bv64,bv64) returns(bool);
+function {:bvbuiltin "bvult"} ult(bv64,bv64) returns(bool);
+function {:bvbuiltin "bvuge"} uge(bv64,bv64) returns(bool);
+function {:bvbuiltin "bvugt"} ugt(bv64,bv64) returns(bool);
 
-function align_value(address : int, value : int, old_value : int, value_mask: int) : int {
+function {:bvbuiltin "bvsle"} sle(bv64,bv64) returns(bool);
+function {:bvbuiltin "bvslt"} slt(bv64,bv64) returns(bool);
+function {:bvbuiltin "bvsge"} sge(bv64,bv64) returns(bool);
+function {:bvbuiltin "bvsgt"} sgt(bv64,bv64) returns(bool);
+
+
+
+function align_value(address : bv64, value : bv64, old_value : bv64, value_mask: bv64) : bv64 {
     bit_or(
             shift_left(
                 bit_and(value, value_mask), 
-                shift_left(bit_and(address, 3), 3)),
-        bit_and(old_value, -shift_left(value_mask, shift_left(bit_and(address, 3), 3))-1))
+                shift_left(bit_and(address, 3bv64), 3bv64)),
+        bit_and(old_value, bit_inv(shift_left(value_mask, shift_left(bit_and(address, 3bv64), 3bv64)))))
 }
 
-function extract_value(address : int, value : int) : int {
+function extract_value(address : bv64, value : bv64) : bv64 {
     shift_right(value, 
-        shift_left(bit_and(address, 3), 3))
+        shift_left(bit_and(address, 3bv64), 3bv64))
 }
 
 
-
-axiom (forall i, m : int :: bit_and(i - bit_and(i,-4),3) == bit_and(i, 3));
-
-axiom (forall i : int :: shift_left(i, 3) == i * 8);
-
-axiom (forall i : int :: shift_left(shift_right(i, 1), 1) == bit_and(i, -2));
-axiom (forall i : int :: shift_left(shift_right(i, 2), 2) == bit_and(i, -4));
-axiom (forall i : int :: shift_left(shift_right(i, 3), 3) == bit_and(i, -8));
-
-//axiom (forall i, m : int :: bit_and(shift_left(i, m), shift_left(7, m)) == shift_left(bit_and(i, 7), m));
-//axiom (forall i, m : int :: bit_and(shift_left(i, m), shift_left(255, m)) == shift_left(bit_and(i, 255), m));
-axiom (forall i, m : int :: bit_and(shift_left(i, m), shift_left(65535, m)) == shift_left(bit_and(i, 65535), m));
-
-axiom (forall a, b, m : int :: (bit_and(a, shift_left(7,m)) == shift_left(b,m)) == (bit_and(shift_right(a,m), 7) == b));
-axiom (forall a, b, m : int :: (bit_and(a, shift_left(255,m)) == shift_left(b,m)) == (bit_and(shift_right(a,m), 255) == b));
-axiom (forall a, b, m : int :: (bit_and(a, shift_left(65535,m)) == shift_left(b,m)) == (bit_and(shift_right(a,m), 65535) == b));
-
-
-axiom (forall a : int :: valid_mask(a, 4294967295) ==> bit_and(a, -4294967295-1) == 0);
-
-
-/*
-axiom (forall a, b, m : int :: bit_and(a, shift_left(7,m)) != shift_left(b,m) && valid_mask(b,7) ==> bit_and(shift_right(a,m), 7) != b);
-axiom (forall a, b, m : int :: bit_and(a, shift_left(255,m)) != shift_left(b,m) && valid_mask(b,255) ==> bit_and(shift_right(a,m), 255) != b);
-axiom (forall a, b, m : int :: bit_and(a, shift_left(65535,m)) != shift_left(b,m) && valid_mask(b,65535) ==> bit_and(shift_right(a,m), 65535) != b);
-*/
-
-
-const max: [int, int] int;
-axiom max == (lambda x, y: int ::
-    if x > y then x else y
+const max: [bv64, bv64] bv64;
+axiom max == (lambda x, y: bv64 ::
+    if uge(x, y) then x else y
 );
 
 
-const min: [int, int] int;
-axiom min == (lambda x, y: int ::
-    if x < y then x else y
+const min: [bv64, bv64] bv64;
+axiom min == (lambda x, y: bv64 ::
+    if ule(x, y) then x else y
 );
 
 
-const add: [int, int] int;
-axiom add == (lambda x, y: int :: x + y);
+const add: [bv64, bv64] bv64;
+axiom add == (lambda x, y: bv64 :: bin_add(x, y));
 
-const sub: [int, int] int;
-axiom sub == (lambda x, y: int :: x - y);
+const sub: [bv64, bv64] bv64;
+axiom sub == (lambda x, y: bv64 :: bin_sub(x, y));
 
-const and: [int, int] int;
-axiom and == (lambda x, y: int :: bit_and(x, y));
+const and: [bv64, bv64] bv64;
+axiom and == (lambda x, y: bv64 :: bit_and(x, y));
 
-const or: [int, int] int;
-axiom or == (lambda x, y: int :: bit_or(x, y));
+const or: [bv64, bv64] bv64;
+axiom or == (lambda x, y: bv64 :: bit_or(x, y));
 
-const xor: [int, int] int;
-axiom xor == (lambda x, y: int :: bit_xor(x, y));
+const xor: [bv64, bv64] bv64;
+axiom xor == (lambda x, y: bv64 :: bit_xor(x, y));
 
-function i2b(i:int) returns (bool) { i != 0 }
-function b2i(b:bool) returns (int) { if b then 1 else 0 }
+function i2b(i:bv64) returns (bool) { i != 0bv64 }
+function b2i(b:bool) returns (bv64) { if b then 1bv64 else 0bv64 }
 
 
 type OrderRelation = [StateIndex, StateIndex, StateIndex, [StateIndex] Ordering, [StateIndex] Effect] bool;
@@ -255,40 +227,37 @@ function no_writes(from, to, write: StateIndex): bool {
     (write < from || to <= write)
 }
 
-function valid_mask(val, mask : int) : bool {
+function valid_mask(val, mask : bv64) : bool {
     val == bit_and(val, mask)
 }
 
-axiom (forall i, m : int :: valid_mask(bit_and(i,m), m));
-axiom (forall i, m : int :: valid_mask(i,m) ==> bit_and(i, -m-1) == 0);
 
-
-type RMWOp = [int, int, int] int;
+type RMWOp = [bv64, bv64, bv64] bv64;
 
 const cmpset, add_op, sub_op, set_op, min_op, max_op, dec_op, inc_op, ret_old: RMWOp;
 
-axiom cmpset == (lambda x, y1, y2 : int :: if x == y1 then y2 else x);
-axiom add_op == (lambda x, y, _: int :: x + y);
-axiom sub_op == (lambda x, y, _: int :: x - y);
-axiom set_op == (lambda x, y, _: int :: y);
-axiom min_op == (lambda x, y, _: int :: if x < y then x else y);
-axiom max_op == (lambda x, y, _: int :: if x < y then y else x);
-axiom dec_op == (lambda x, _1, _2: int :: x-1);
-axiom inc_op == (lambda x, _1, _2: int :: x+1);
+axiom cmpset == (lambda x, y1, y2 : bv64 :: if x == y1 then y2 else x);
+axiom add_op == (lambda x, y, _: bv64 :: bin_add(x, y));
+axiom sub_op == (lambda x, y, _: bv64 :: bin_sub(x, y));
+axiom set_op == (lambda x, y, _: bv64 :: y);
+axiom min_op == (lambda x, y, _: bv64 :: min[x, y]);
+axiom max_op == (lambda x, y, _: bv64 :: max[x, y]);
+axiom dec_op == (lambda x, _1, _2: bv64 :: bin_sub(x, 1bv64));
+axiom inc_op == (lambda x, _1, _2: bv64 :: bin_add(x, 1bv64));
 
-axiom ret_old == (lambda x, _1, _2 : int :: x);
+axiom ret_old == (lambda x, _1, _2 : bv64 :: x);
 
 const bit8, bit16 : [RMWOp] RMWOp;
-axiom bit8 == (lambda op : RMWOp :: (lambda x, y1, y2 : int :: op[x, bit_and(y1,255), bit_and(y2, 255)]));
-axiom bit16 == (lambda op : RMWOp :: (lambda x, y1, y2 : int :: op[x, bit_and(y1,65535), bit_and(y2, 65535)]));
+axiom bit8 == (lambda op : RMWOp :: (lambda x, y1, y2 : bv64 :: op[x, bit_and(y1,255bv64), bit_and(y2, 255bv64)]));
+axiom bit16 == (lambda op : RMWOp :: (lambda x, y1, y2 : bv64 :: op[x, bit_and(y1,65535bv64), bit_and(y2, 65535bv64)]));
 
-type AwaitOp = [int, int] bool;
+type AwaitOp = [bv64, bv64] bool;
 
 const eq, neq, lt, le, gt, ge: AwaitOp;
 
-axiom eq  == (lambda x, y: int :: x == y);
-axiom neq == (lambda x, y: int :: x != y);
-axiom lt  == (lambda x, y: int :: x <  y);
-axiom le  == (lambda x, y: int :: x <= y);
-axiom gt  == (lambda x, y: int :: x >  y);
-axiom ge  == (lambda x, y: int :: x >= y);
+axiom eq  == (lambda x, y: bv64 :: x == y);
+axiom neq == (lambda x, y: bv64 :: x != y);
+axiom lt  == (lambda x, y: bv64 :: ult(x, y));
+axiom le  == (lambda x, y: bv64 :: ule(x, y));
+axiom gt  == (lambda x, y: bv64 :: ugt(x, y));
+axiom ge  == (lambda x, y: bv64 :: uge(x, y));
